implemented balance query, cleaned

main/Syntax.v
@@ -1,22 +1,45 @@
-Require Import ZArith.
-Require Import List.
-
-Require Import String.
+Require Export ZArith.
+Require Export String.
+Require Export List.
 
 Open Scope string_scope.
+Open Scope Z_scope.
 
-(* TODO use modules, for balance, envs, etc *)
+
+(**************************************************************)
+(** Solidity address *)
+
+Definition address := string.
+Definition address_payable := address.
+
+Definition Default_Address := "default_address".
+
+(*
+ *
+ TODO Consider better separation for address i.e.:
+Inductive address :=
+| Address : string -> address
+| Address_Payable : string -> address
+.
+*)
 
 
-(** Basic types *)
-
+(**************************************************************)
+(** Integers *)
+ 
 Inductive aexp :=
 | Int : Z -> aexp
 | AId : string -> aexp
 | Plus : aexp -> aexp -> aexp
 | Mul : aexp -> aexp -> aexp
 | Div : aexp -> aexp -> aexp
-| Rem : aexp -> aexp -> aexp.
+| Rem : aexp -> aexp -> aexp
+| BalanceOf : address -> aexp.
+
+Definition Default_Aexp := Int 0.
+
+(**************************************************************)
+(** Bool *)
 
 Inductive bexp :=
 | Boolean : bool -> bexp
@@ -30,17 +53,22 @@ Inductive bexp :=
 | And : bexp -> bexp -> bexp
 | Or : bexp -> bexp -> bexp.
 
-
-Definition Default_Aexp := Int 0.
 Definition Default_Bexp := Boolean false.
 
 
-(** Solidity address *)
+(** Message *)
 
-Definition address := string.
-Definition address_payable := string.
+Record msg :=
+mkMsg {
+value : Z;
+sender : address_payable
+}.
+
+Definition Default_Msg := {| value := 0;
+                             sender := Default_Address |}.
 
 
+(**************************************************************)
 (** Statements *)
 
 Inductive instr :=
@@ -55,77 +83,99 @@ Inductive instr :=
 | Transfer : address_payable -> aexp -> instr.
 
 
-Inductive function_body :=
-| Body : list instr -> function_body
-| EmptyBody : function_body.
+(**************************************************************)
+(** * Environments *)
+
+Definition Env T1 T2 := T1 -> option T2.
+
+
+(** aexp *)
+
+Definition Aexp_Env := Env string Z.
+Definition Empty_Aexp_Env : Aexp_Env := fun x => None.
+
+Definition update_aexp (env : Aexp_Env) (var : option string) (val : Z) : Aexp_Env :=
+  fun x => match var with
+  | Some str => if (string_dec x str) then Some val
+                else (env x)
+  | _ => None
+  end.
+
+
+(** bexp *)
+
+Definition Bexp_Env := Env string bool.
+Definition Empty_Bexp_Env : Bexp_Env := fun x => None.
+
+Definition declare_bexp (ident : string) : Bexp_Env :=
+  fun x => if (string_dec x ident) then Some false
+           else None.
+
+Definition update_bexp (env : Bexp_Env) (var : string) (val : bool) : Bexp_Env :=
+  fun x => if (string_dec x var) then Some val
+  else (env x).
+
+
+(** contract functions *)
 
 Definition Code := list instr.
 
+Inductive function_body :=
+| Body : Code -> function_body
+| EmptyBody : function_body.
 
-(** Environment *)
-
-Definition Env (T : Type) := string -> option T.
-
-Definition Aexp_Env := Env Z.
-Definition Empty_Aexp_Env : Aexp_Env := fun x => None.
-
-Definition Bexp_Env := Env bool.
-Definition Empty_Bexp_Env : Bexp_Env := fun x => None.
-
-Definition Functions_Env := Env function_body.
+Definition Functions_Env := Env string function_body.
 Definition Empty_Functions_Env : Functions_Env := fun x => None.
 
+Definition defineFunction (env : Functions_Env) (name : string) (body : function_body) : Functions_Env :=
+  fun x => if (string_dec x name) then Some body
+  else (env x).
 
-(** Contract balances *)
-
-Definition BalanceMap := address -> Z.
-Definition Empty_BalanceMap : BalanceMap := fun a => 0%Z.
-
-Definition updateBalance (map : BalanceMap) (addr : address) (amount : Z) : address -> Z :=
-fun a' => if string_dec addr a' then amount else map a'.
-
-
-
-(** Message structure *)
-
-Record msg :=
-mkMsg {
-value : Z;
-sender : address_payable
-}.
-
-Definition Default_Msg := {| value := 0%Z;
-                             sender := "default_sender" |}.
+Definition getFunctionCode (opt_body : option function_body) : Code :=
+  match opt_body with
+  | Some (Body code) => code
+  | _ => nil
+  end.
 
 
-(** Function scope *)
+(** balances *)
+
+Definition Balance_Env := Env address Z.
+Definition Empty_BalanceEnv : Balance_Env := fun a => None.
+
+Definition updateBalance (map : Balance_Env) (addr : address) (amount : Z) : Balance_Env :=
+fun a' => if string_dec addr a' then Some amount else map a'.
+
+
+(** function locals *)
 
 Record FunctionEnv :=
 mkEnv {
  aexp_env : Aexp_Env;
  bexp_env : Bexp_Env;
  next_code : Code;
- balance_map : BalanceMap;
  msg_data : msg
 }.
 
+Definition Empty_FunctionEnv := {| aexp_env := Empty_Aexp_Env;
+                                bexp_env := Empty_Bexp_Env;
+                                next_code := nil;
+                                msg_data := Default_Msg |}.
+
 Definition replace_aexp_env := 
-fun (fenv : FunctionEnv) (new_env : Aexp_Env) => mkEnv new_env (bexp_env fenv) (next_code fenv) (balance_map fenv) (msg_data fenv).
+fun (fenv : FunctionEnv) (new_env : Aexp_Env) => mkEnv new_env (bexp_env fenv) (next_code fenv) (msg_data fenv).
 
 Definition replace_bexp_env := 
-fun (fenv : FunctionEnv) (new_env : Bexp_Env) => mkEnv (aexp_env fenv) new_env (next_code fenv) (balance_map fenv) (msg_data fenv).
+fun (fenv : FunctionEnv) (new_env : Bexp_Env) => mkEnv (aexp_env fenv) new_env (next_code fenv) (msg_data fenv).
 
 Definition replace_next_code := 
-fun (fenv : FunctionEnv) (new_next_code : Code) => mkEnv (aexp_env fenv) (bexp_env fenv) new_next_code (balance_map fenv) (msg_data fenv).
-
-Definition replace_bmap := 
-fun (fenv : FunctionEnv) (bmap : BalanceMap) => mkEnv (aexp_env fenv) (bexp_env fenv) (next_code fenv) bmap (msg_data fenv).
+fun (fenv : FunctionEnv) (new_next_code : Code) => mkEnv (aexp_env fenv) (bexp_env fenv) new_next_code (msg_data fenv).
 
 Definition replace_msg_data := 
-fun (fenv : FunctionEnv) (new_msg : msg) => mkEnv (aexp_env fenv) (bexp_env fenv) (next_code fenv) (balance_map fenv) new_msg.
+fun (fenv : FunctionEnv) (new_msg : msg) => mkEnv (aexp_env fenv) (bexp_env fenv) (next_code fenv) new_msg.
 
 
-(** Contract scope *)
+(** Contract state *)
 
 Record ContractState :=
 mkContractState {
@@ -140,38 +190,51 @@ fun (cstate : ContractState) (new_env : Aexp_Env)
  => mkContractState (c_address cstate) (fn_env cstate) new_env (bexp_vars cstate).
 
 
-Definition Default_Address := "default_address".
-
 Definition Default_ContractState := {| c_address := Default_Address;
                                        fn_env := Empty_Functions_Env;
                                        aexp_vars := Empty_Aexp_Env;
                                        bexp_vars := Empty_Bexp_Env |}.
 
-Definition Empty_FunctionEnv := {| aexp_env := Empty_Aexp_Env;
-                                bexp_env := Empty_Bexp_Env;
-                                next_code := nil;
-                                balance_map := Empty_BalanceMap;
-                                msg_data := Default_Msg |}.
 
-
-(** Environment utils *)
-
-Definition defineFunction (env : Functions_Env) (name : string) (body : function_body) : Functions_Env :=
-  fun x => if (string_dec x name) then Some body
-  else (env x).
-
-Definition getFunctionCode (opt_body : option function_body) : Code :=
-  match opt_body with
-  | Some (Body code) => code
-  | _ => nil
-  end.
-
+(**************************************************************)
+(** Contracts Env *)
 
 Definition ContractsEnv := address -> ContractState.
 Definition Empty_ContractsEnv : ContractsEnv := fun x => Default_ContractState.
+
 Definition updateContractsEnv (env : ContractsEnv) (addr : address) (state : ContractState) : ContractsEnv :=
   fun x => if (string_dec x addr) then state
   else (env x).
+
+Definition get_calling_contract (opt_addr : option address) (env : ContractsEnv) (current_contract : ContractState) :=
+match opt_addr with
+| Some v => env v
+| _ => current_contract
+end.
+
+
+(**************************************************************)
+(** More unfold/unpack helpers *)
+
+(* * More generic *)
+(* 
+Definition unfold_option {T1} {T2} (opt : option T1) (default : T2) (t1_to_t2 : T1 -> T2) : T2 :=
+match opt with
+| Some t1 => t1_to_t2 t1
+| _ => default
+end.
+*)
+
+
+Definition unfold_option {T} (opt : option T) (default : T) : T :=
+match opt with
+| Some v => v
+| _ => default
+end.
+
+Definition unfold_option_z := fun opt => unfold_option opt 0.
+Definition unfold_option_bool := fun opt => unfold_option opt false.
+
 
 Definition unfold_aexp_literal (e : aexp) : option Z :=
 match e with
@@ -179,7 +242,16 @@ match e with
 | _ => None
 end.
 
-Check unfold_aexp_literal.
+
+Definition unfold_aexp_id (e : aexp) : option string :=
+match e with
+| AId s => Some s
+| _ => None
+end.
+
+
+(**************************************************************)
+(** Declaration of aexp *)
 
 Fixpoint declareAexpList (env : Aexp_Env) (decl_pairs : list (string * option aexp)) : Aexp_Env :=
 fun x => match decl_pairs with
@@ -192,144 +264,103 @@ fun x => match decl_pairs with
                   else declareAexpList env rest x
 end.
 
-Definition update_aexp (env : Aexp_Env) (var : option string) (val : Z) : Aexp_Env :=
-  fun x => match var with
-  | Some str => if (string_dec x str) then Some val
-                else (env x)
-  | _ => None
-  end.
 
-(* 
-Definition unfold_option {T1} {T2} (opt : option T1) (default : T2) (t1_to_t2 : T1 -> T2) : T2 :=
-match opt with
-| Some t1 => t1_to_t2 t1
-| _ => default
-end.
- *)
+(**************************************************************)
+(** * Evaluation of expressions *)
 
-Definition unfold_option {T} (opt : option T) (default : T) : T :=
-match opt with
-| Some v => v
-| _ => default
-end.
+(** aexp *)
 
-
-Definition unfold_aexp_id (e : aexp) : option string :=
-match e with
-| AId s => Some s
-| _ => None
-end.
-
-
-Definition unfold_option_z := fun opt => unfold_option opt 0%Z.
-Definition unfold_option_bool := fun opt => unfold_option opt false.
-
-Fixpoint eval_aexp (env : Aexp_Env) (a : aexp) : option Z :=
+Fixpoint eval_aexp (env : Aexp_Env) (bm : Balance_Env) (a : aexp) : option Z :=
   match a with
   | Int z => Some z
   | AId x => env x
-  | Plus a1 a2 => match (eval_aexp env a1), (eval_aexp env a2) with
+  | BalanceOf x => bm x
+  | Plus a1 a2 => match (eval_aexp env bm a1), (eval_aexp env bm a2) with
                   | Some v1, Some v2 => Some (Z.add v1 v2)
                   | _, _ => None
                   end
-  | Mul a1 a2 => match (eval_aexp env a1), (eval_aexp env a2) with
+  | Mul a1 a2 => match (eval_aexp env bm a1), (eval_aexp env bm a2) with
                   | Some v1, Some v2 => Some (Z.mul v1 v2)
                   | _, _ => None
                   end
-  | Div a1 a2 => match (eval_aexp env a1), (eval_aexp env a2) with
+  | Div a1 a2 => match (eval_aexp env bm a1), (eval_aexp env bm a2) with
                  | Some v1, Some v2 => if (Z.eqb 0 v2) then None else Some (Z.div v1 v2)
                  | _, _ => None
                  end
-  | Rem a1 a2 => match (eval_aexp env a1), (eval_aexp env a2) with
+  | Rem a1 a2 => match (eval_aexp env bm a1), (eval_aexp env bm a2) with
                  | Some v1, Some v2 => if (Z.eqb 0 v2) then None else Some (Z.rem v1 v2)
                  | _, _ => None
                  end
   end.
 
 
-Definition unfold_opt_aexp (opt_aexp : option aexp) (env : Aexp_Env) : option Z :=
+Definition unfold_opt_aexp (opt_aexp : option aexp) (env : Aexp_Env) (bm : Balance_Env) : option Z :=
 match opt_aexp with
-| Some v => eval_aexp env v
+| Some v => eval_aexp env bm v
 | _ => None
 end.
 
 
+(** * Some proof examples *)
+
 Example unknown_id_evals_none:
-  eval_aexp Empty_Aexp_Env (AId "a") = None.
+  eval_aexp Empty_Aexp_Env Empty_BalanceEnv (AId "a") = None.
 Proof.
   reflexivity.
 Qed.
 
 Example zero_division:
-  eval_aexp Empty_Aexp_Env (Div (Int 1) (Int 0)) = None.
+  eval_aexp Empty_Aexp_Env Empty_BalanceEnv (Div (Int 1) (Int 0)) = None.
 Proof.
   reflexivity.
 Qed.
 
 Example zero_division_remainder:
-  eval_aexp Empty_Aexp_Env (Rem (Int 1) (Int 0)) = None.
+  eval_aexp Empty_Aexp_Env Empty_BalanceEnv (Rem (Int 1) (Int 0)) = None.
 Proof.
   reflexivity.
 Qed.
 
-Definition declare_bexp (ident : string) : Bexp_Env :=
-  fun x => if (string_dec x ident) then Some false
-           else None.
 
-Definition update_bexp (env : Bexp_Env) (var : string) (val : bool) : Bexp_Env :=
-  fun x => if (string_dec x var) then Some val
-  else (env x).
+(** bexp *)
 
-Fixpoint eval_bexp (aexp_env : Aexp_Env) (bexp_env : Bexp_Env) (b : bexp) : option bool :=
+Fixpoint eval_bexp (aexp_env : Aexp_Env) (bm : Balance_Env) (bexp_env : Bexp_Env) (b : bexp) : option bool :=
   match b with
   | Boolean b' => Some b'
   | BId x => bexp_env x
-  | Aexp_Lt a1 a2 => match (eval_aexp aexp_env a1), (eval_aexp aexp_env a2) with
+  | Aexp_Lt a1 a2 => match (eval_aexp aexp_env bm a1), (eval_aexp aexp_env bm a2) with
                     | Some v1, Some v2 => Some (Z.ltb v1 v2)
                     | _, _ => None
                     end
-  | Aexp_Leq a1 a2 => match (eval_aexp aexp_env a1), (eval_aexp aexp_env a2) with
+  | Aexp_Leq a1 a2 => match (eval_aexp aexp_env bm a1), (eval_aexp aexp_env bm a2) with
                     | Some v1, Some v2 => Some (Z.leb v1 v2)
                     | _, _ => None
                     end
-  | Aexp_Eq a1 a2 => match (eval_aexp aexp_env a1), (eval_aexp aexp_env a2) with
+  | Aexp_Eq a1 a2 => match (eval_aexp aexp_env bm a1), (eval_aexp aexp_env bm a2) with
                     | Some v1, Some v2 => Some (Z.eqb v1 v2)
                     | _, _ => None
                     end
-  | Aexp_Geq a1 a2 => match (eval_aexp aexp_env a1), (eval_aexp aexp_env a2) with
+  | Aexp_Geq a1 a2 => match (eval_aexp aexp_env bm a1), (eval_aexp aexp_env bm a2) with
                     | Some v1, Some v2 => Some (Z.geb v1 v2)
                     | _, _ => None
                      end
-  | Aexp_Gt a1 a2 => match (eval_aexp aexp_env a1), (eval_aexp aexp_env a2) with
+  | Aexp_Gt a1 a2 => match (eval_aexp aexp_env bm a1), (eval_aexp aexp_env bm a2) with
                     | Some v1, Some v2 => Some (Z.gtb v1 v2)
                     | _, _ => None
                     end
-  | Not b' => match (eval_bexp aexp_env bexp_env b') with
+  | Not b' => match (eval_bexp aexp_env bm bexp_env b') with
               | Some b'' => Some (negb b'')
               | _ => None
               end
-  | And b1 b2 => match (eval_bexp aexp_env bexp_env b1), (eval_bexp aexp_env bexp_env b2) with
+  | And b1 b2 => match (eval_bexp aexp_env bm bexp_env b1), (eval_bexp aexp_env bm bexp_env b2) with
                  | Some b1', Some b2' => Some (andb b1' b2')
                  | _, _ => None
                  end
-  | Or b1 b2 => match (eval_bexp aexp_env bexp_env b1), (eval_bexp aexp_env bexp_env b2) with
+  | Or b1 b2 => match (eval_bexp aexp_env bm bexp_env b1), (eval_bexp aexp_env bm bexp_env b2) with
                  | Some b1', Some b2' => Some (orb b1' b2')
                  | _, _ => None
                  end
   end.
-
-
-Definition get_calling_contract (opt_addr : option address) (env : ContractsEnv) (current_contract : ContractState) :=
-match opt_addr with
-| Some v => env v
-| _ => current_contract
-end.
-
-
-
-
-
-
 
 
 
